WIP

theories/AAC_hetero.v
@@ -2,8 +2,8 @@
 (*  This is part of aac_tactics, it is distributed under the terms of the  *)
 (*         GNU Lesser General Public License version 3                     *)
 (*              (see file LICENSE for more details)                        *)
-(*                                                                         *)
-(*       Copyright 2018: Fabian Kunze.                                     *)
+(*       Copyright 2009-2010: Thomas Braibant, Damien Pous.                *)
+(*                      2018: Fabian Kunze.                                *)
 (***************************************************************************)
 
 (** * Theory file for the aac_apply tactic
@@ -20,6 +20,10 @@
 
    This currently just handles equality as relation.
 
+   It is able to handle operations that are associative, but not homogeneous, as e.g. function composition or arrow composition in category theory.
+   Therefore, every type involved is seen as an category: There are 'objects' and 'arrows'.
+   For homogenous types, on can e.g. use Unit as object Type.
+
    It handles assoc/commutaive functions over different types, but each function must be homogeneous (of shape X -> X -> X) *)
 
 Require Import Utils.
@@ -32,16 +36,23 @@ Local Open Scope list_scope.
 
 
 Set Implicit Arguments.
-Set Asymmetric Patterns.
 
 
 Module ReifH.
   Section ReifH.
     (* We use environments to store the various operators and the
      morphisms.*)
+    Local Notation idC := nat.
+    Local Notation idT := ((idC * idx * idx)%type).
+    
+    Lemma idT_eq_dec (x y : idT): {x = y} + {x <> y}.
+    Proof.
+      repeat decide equality.
+    Qed.
 
-    Local Notation idT := nat.
-    Variable l_type : nelist Type.
+    Local Hint Resolve idT_eq_dec.
+    
+    Variable l_type : nelist {obj : idx -> Type & idx -> idx -> Type}. (* The different kinds of types supported on various levels*)
 
     Fixpoint nthne X n (l:nelist X) {struct l}: X :=
       match l,n with
@@ -50,7 +61,7 @@ Module ReifH.
       | consne _ l,S n => nthne n l
       end. 
     
-    Let e_type := (fun i => nthne i l_type).
+    Let e_type := (fun (i:idT) => let '(i,l,r):= i in (projT2 (nthne i l_type)) l r).
 
     (* TODO: e_rel for different relations?*)
     (*Variable e_rel : forall iTy, e_type iTy -> e_type iTy -> Prop.*)
@@ -76,60 +87,84 @@ Module ReifH.
     (** ** binary operations *)
 
     Section Bin.
-      Record Bin iTy :=
+      Record Bin iCat :=
         mkBin {
-            bin_value: e_type iTy -> e_type iTy -> e_type iTy;
-            bin_assoc: Associative eq bin_value;
-            bin_comm: option (Commutative eq bin_value)
+            (* order: as in fuction composition*)
+            bin_value: forall iObj1 iObj2 iObj3, e_type (iCat,iObj2,iObj3)
+                                -> e_type (iCat,iObj1,iObj2)
+                                -> e_type (iCat,iObj1,iObj3);
+            bin_assoc: HAssociative (fun _ _ => eq) (bin_value);
+            bin_comm: option (HCommutative (fun _ _ => eq) bin_value)
           }.
     End Bin.
     
     Arguments bin_value : clear implicits.
-    Arguments bin_value {iTy} _.
+    Arguments bin_value {iCat} _.
 
     Variable e_sym: forall iTy, idx -> Sym iTy.
-    Variable e_bin: forall iTy, idx -> Bin iTy.
+    Variable e_bin: forall iCat, idx -> Bin iCat.
 
     (** packaging units (depends on e_bin) *)
 
-    Record unit_of iTy (u:e_type iTy) :=
+    Record unit_of iCat (u:forall iObj, e_type (iCat,iObj,iObj)) :=
       mk_unit_for {
           uf_iBin: idx;
-          uf_bin := e_bin iTy uf_iBin;
-          uf_desc: Unit (@eq _) (bin_value uf_bin) u
+          uf_bin := e_bin iCat uf_iBin;
+          uf_desc: HUnit (fun _ _ => @eq _) (bin_value uf_bin) u
         }.
 
 
-    Record unit_pack iTy :=
+    Record unit_pack iCat :=
       mk_unit_pack {
-          u_value:> e_type iTy;
+          u_value:> (forall iObj, e_type (iCat,iObj,iObj));
           u_desc: list (unit_of _ u_value)
         }.
-    Variable e_unit: forall iTy, idx -> unit_pack iTy.
+    Variable e_unit: forall iCat, idx -> unit_pack iCat.
 
-    Inductive T: idT -> Type :=
-    | sum iTy (i : idx): mset (T iTy) -> T iTy
-    | prd iTy: idx -> nelist (T iTy) -> T iTy
-    | sym iTy (i : idx):
-             vT (sym_args (e_sym iTy i)) -> T iTy
-    | unit iTy (j:idx): T iTy
+    Inductive T: idC -> idx -> idx -> Type :=
+    | sum {Cat A} (i : idx): mset (T Cat A A) -> T Cat A A
+    | prd {Cat A B}: idx -> vAT Cat A B -> T Cat A B
+    | sym {Cat A B} (i : idx):
+        vT (sym_args (e_sym (Cat,A,B) i)) -> T Cat A B
+    | unit {Cat} {A} (j:idx): T Cat A A
     with vT: list idT -> Type :=
          | vnil: vT nil
-         | vcons X ar: T X -> vT ar -> vT (X::ar).
+         | vcons {Cat A B} ar: T Cat A B -> vT ar -> vT ((Cat,A,B)::ar)
+    with vAT: idC -> idx -> idx -> Type := (* nonempty vector of arrows whose objects match at the border, for assoc *)
+         | vAnil {Cat A B} : T Cat A B -> vAT Cat A B
+         | vAcons {Cat A B C} : T Cat B C -> vAT Cat A B -> vAT Cat A C.
 
-    (** lexicographic rpo over the normalised syntax *)
-    Fixpoint compare {iTy jTy} (u: T iTy) (v: T jTy) :=
+    Fixpoint vAapp {Cat A B C} (l: vAT Cat B C) : vAT Cat A B -> vAT Cat A C :=
+      match l with
+        vAnil x => fun A l' => vAcons x l'
+      | vAcons t q => fun A l' => vAcons t (vAapp q l')
+      end A.
+
+    Section fold_map_vA.
+      Variable F : idC -> idx -> idx -> Type.
+      Variable ret : forall Cat A B, T Cat A B -> F Cat A B.
+      Variable bind : forall Cat A B C, T Cat B C -> F Cat A B -> F Cat A C.
+      Fixpoint fold_map_vA {Cat A B} (l : vAT Cat A B) : F Cat A B :=
+        match l with
+        | vAnil x => ret x
+        | @vAcons Cat A B C u l =>  bind u (fold_map_vA l)
+        end.
+    End fold_map_vA.
+    
+
+    (** lexicographic rpo over the normalised syntax *) (* does implicitly assume that Cat A B = Cat' A' B', but that is not important for us *)
+    Fixpoint compare {Cat A B Cat' A' B'} (u: T Cat A B) (v: T Cat' A' B') :=
       match u,v with
-      | sum iTy i l, sum _ j vs => lex (idx_compare i j) (mset_compare compare l vs)
-      | prd iTy i l, prd _ j vs => lex (idx_compare i j) (list_compare compare l vs)
-      | sym iTy i l, sym jTy j vs => lex (idx_compare i j) (vcompare l vs)
-      | unit _ i , unit _ j => (idx_compare i j)
-      | unit _ _ , _        => Lt
-      | _      , unit _ _  => Gt
-      | sum _ _ _, _        => Lt
-      | _      , sum _ _ _  => Gt
-      | prd _ _ _, _        => Lt
-      | _      , prd _ _ _  => Gt
+      | sum i l, sum j vs => lex (idx_compare i j) (mset_compare compare l vs)
+      | prd i l, prd j vs => lex (idx_compare i j) (vAcompare l vs)
+      | sym i l, sym j vs => lex (idx_compare i j) (vcompare l vs)
+      | unit i , unit j => (idx_compare i j)
+      | unit _ , _    => Lt
+      | _      , unit _  => Gt
+      | sum _ _, _        => Lt
+      | _      , sum _ _  => Gt
+      | prd _ _, _        => Lt
+      | _      , prd _ _  => Gt
 
       end
     with vcompare {ar1 ar2} (us: vT ar1) (vs: vT ar2) :=
@@ -137,50 +172,95 @@ Module ReifH.
            | vnil, vnil => Eq
            | vnil, _  => Lt
            | _,   vnil => Gt
-           | vcons _ _ u us, vcons _ _ v vs => lex (compare u v) (vcompare us vs)
+           | vcons  u us, vcons v vs => lex (compare u v) (vcompare us vs)
+           end
+    with vAcompare {Cat A B Cat' A' B'} (us: vAT Cat A B) (vs: vAT Cat' A' B') :=
+           match us,vs with
+           | vAnil u, vAnil v => compare u v
+           | vAnil _, _  => Lt
+           | _,  vAnil _ => Gt
+           | @vAcons _ _ C _ u us, @vAcons _ _ C' _ v vs => lex (idx_compare C C') (lex (compare u v) (vAcompare us vs))
            end.
 
     (** ** Evaluation from syntax to the abstract domain *)
 
-    Fixpoint eval {iTy} (u : T iTy) : (e_type iTy) :=
+    Fixpoint eval {Cat A B} (u : T Cat A B) : (e_type (Cat,A,B)) :=
       match u with
-      | sum iTy i l => let o := bin_value (e_bin iTy i) in
+      | @sum Cat A iBin l => let o := bin_value (e_bin _ iBin) A A A in
                   fold_map (fun un => let '(u,n):=un in @copy _ o n (eval u)) o l
-      | prd iTy i l => fold_map eval (bin_value (e_bin iTy i)) l
-      | sym iTy i v => eval_aux v (sym_value (e_sym iTy i))
-      | unit iTy i  => e_unit iTy i
+      | prd iBin l => vaeval iBin l
+      | @sym Cat A B i v => eval_aux v (sym_value (e_sym (Cat,A,B) i))
+      | @unit Cat A i  => u_value (e_unit Cat i) A
       end
-    with eval_aux {ar iTy} (v: vT ar): type_of_ar ar iTy -> e_type iTy :=
+    with eval_aux {ar Cat A B} (v: vT ar): type_of_ar ar (Cat,A,B) -> e_type (Cat,A,B) :=
            match v with
            | vnil  => fun f => f
-           | vcons X ar x v => fun f => eval_aux v (f (eval x))
+           | vcons x v => fun f => eval_aux v (f (eval x))
+           end
+    with vaeval {Cat A B} iBin (vs: vAT Cat A B): e_type (Cat,A,B) :=
+           match vs with
+           | vAnil u => eval u
+           | @vAcons Cat _ _ _ u us => bin_value (e_bin Cat iBin) _ _ _ (eval u) (vaeval iBin us)
            end.
-
 
     (** we need to show that compare reflects equality (this is because
      we work with msets rather than lists with arities) *)
-    Lemma tcompare_weak_spec: forall iTy (u v : T iTy), compare_weak_spec u v (compare u v)
+    Lemma tcompare_weak_spec: forall Cat A B (u v : T Cat A B), compare_weak_spec u v (compare u v)
+    with vAtcompare_weak_spec: forall Cat A B (u v : vAT Cat A B), compare_weak_spec u v (vAcompare u v)
     with vcompare_reflect_eqdep: forall ar us ar' vs (H: ar=ar'), vcompare us vs = Eq -> cast vT H us = vs.
     Proof.
-      -destruct u. 
-       +destruct v; simpl; try constructor.
-        case (pos_compare_weak_spec i i0); intros; try constructor.
-        case (mset_compare_weak_spec compare (tcompare_weak_spec iTy) m m0); intros; try constructor.
-       +destruct v; simpl; try constructor.
-        case (pos_compare_weak_spec p p0); intros; try constructor.
-        case (list_compare_weak_spec compare (tcompare_weak_spec iTy) n n0); intros; try constructor.
-       +intros u. destruct u. 1,2,4:now constructor. cbn.
-        destruct (pos_compare_weak_spec i i0); intros; try constructor.   
-        case_eq (vcompare v v0); intro Hv; try constructor.
+      -intros Cat A B [].
+       +intros v. refine (match v as v' in T Cat' A' B' return forall H : Cat' A' B' = _,
+                   compare_weak_spec _ (cast _ H v') (compare _ v') with
+               | sum _ _ => _
+               | _ => _
+                          end eq_refl). all:intros H;try constructor.
+        inversion H;subst. cbn. rewrite cast_eq. 2:trivial. 
+        case (pos_compare_weak_spec i p0); intros; try constructor.
+        case (mset_compare_weak_spec compare (tcompare_weak_spec _) m m0); intros; try constructor.
+       +intros v0. refine (match v0 as v' in T Cat' A' B' return forall H : Cat' A' B' = _,
+                   compare_weak_spec _ (cast _ H v') (compare _ v') with
+               | sum _ _ => _
+               | _ => _
+                          end eq_refl). all:intros H;try constructor.
+        inversion H;subst. cbn.  
+        case (pos_compare_weak_spec p p1); intros; try constructor.
+        case (vAtcompare_weak_spec _ v v1);intros;try constructor.  
+       +intros v0. refine (match v0 as v' in T Cat' A' B' return forall H : Cat' A' B' = _,
+                   compare_weak_spec _ (cast _ H v') (compare _ v') with
+               | sum _ _ => _
+               | _ => _
+                          end eq_refl). all:intros H;try constructor.
+        inversion H;subst. cbn.  
+        destruct (pos_compare_weak_spec i p0); intros; try constructor.   
+        case_eq (vcompare v v1); intro Hv; try constructor.
         rewrite <- (vcompare_reflect_eqdep _ _ _ _ eq_refl Hv). cbn. constructor.
-       +intros []. 1,2,3:now constructor. cbn.
-        case (pos_compare_weak_spec j j0); intros; try constructor. 
+       +intros v0. refine (match v0 as v' in T Cat' A' B' return forall H : Cat' A' B' = _,
+                   compare_weak_spec _ (cast _ H v') (compare _ v') with
+               | sum _ _ => _
+               | _ => _
+                          end eq_refl). all:intros H;try constructor.
+        inversion H;subst. rewrite cast_eq. 2:trivial. cbn.
+        case (pos_compare_weak_spec j p0); intros; try constructor. 
+      -intros Cat A B [] v0.
+       +destruct v0;intros;try constructor. cbn.
+        case (tcompare_weak_spec _ t t0). all:intros;constructor.
+       +refine (match v0 as v0 in vAT Cat' A' B' return forall H : Cat' A' B' = _,
+                   compare_weak_spec _ (cast (fun Cat A B => vAT Cat A B) H v0) (vAcompare _ v0) with
+               | vAnil _ => _
+               | _ => _
+                          end eq_refl). all:intros H;try constructor. 
+        inversion H;subst. cbn. rewrite cast_eq. 2:trivial. revert v1.
+        revert dependent B. intros B.
+        revert dependent p0. intros p0. case_eq (pos_compare_weak_spec B p0);intros;try constructor. 
+        case (tcompare_weak_spec _ t t0);intros;try constructor.
+        case (vAtcompare_weak_spec _ v v1);intros;constructor. 
       -induction us; destruct vs; simpl; intros H Huv; try discriminate.
-       +apply cast_eq, list_eq_dec, Nat.eq_dec.
+       +apply cast_eq, list_eq_dec, idT_eq_dec.
        +inversion H. subst.
         revert Huv. case (tcompare_weak_spec _ t t0). 2,3:easy.
         intro. intros H'. apply IHus with (H:=eq_refl) in H'. cbn in H'. subst.
-        apply cast_eq,list_eq_dec,Nat.eq_dec. 
+        apply cast_eq,list_eq_dec,idT_eq_dec. 
     Qed.
     (*
     Instance eval_aux_compat i (l: vT i): Proper (sym.rel_of X R i ==> R) (eval_aux l).
@@ -191,77 +271,73 @@ Module ReifH.
     Qed.
      *)
     
-  (* in type iTy, is i a unit for [j] ? *)
-  Definition is_unit_of iTy j i :=
-    List.existsb (fun p => eq_idx_bool j (uf_iBin p)) (u_desc (e_unit iTy i)).
+  (* in type Cat, is i a unit for [j] ? *)
+  Definition is_unit_of Cat j i :=
+    List.existsb (fun p => eq_idx_bool j (uf_iBin p)) (u_desc (e_unit Cat i)).
 
   (* is [iTY i] commutative ? *)
-  Definition is_commutative iTy i :=
-    match bin_comm (e_bin iTy i) with Some _ => true | None => false end.
+  Definition is_commutative Cat i :=
+    match bin_comm (e_bin Cat i) with Some _ => true | None => false end.
 
 
   (** ** Normalisation *)
 
-  Inductive discr {A} : Type :=
-  | Is_op : A -> discr
-  | Is_unit : idx -> discr
-  | Is_nothing : discr .
+  Inductive discr {A}: idT -> Type :=
+  | Is_op Cat A B (m: A): discr Cat A B
+  | Is_unit Cat A: idx -> discr (Cat,(A,A))
+  | Is_nothing Cat A B: discr Cat A B.
  
   (* This is called sum in the std lib *)
-  Inductive m {A} {B} :=
-  | left : A -> m
-  | right : B -> m.
 
   (* combine intro rhs *)
-  Definition comp A B (merge : B -> B -> B) (l : B) (l' : @m A B) : @m A B :=
+  Definition comp A B (merge : B -> B -> B) (l : B) (l' : A + B) : A + B :=
     match l' with
-      | left _ => right l
-      | right l' => right (merge l l')
+      | inl _ => inr l
+      | inr l' => inr (merge l l')
     end.
  
   (** auxiliary functions, to clean up sums  *)
 
   Section sums.
-    Variable iTy : idT. (* index of the Type to look at *)
     Variable i : idx. (* index of binary function to normalise *)
     Variable is_unit : idx -> bool.
 
 
-    Definition sum' (u: mset (T iTy)): T iTy :=
+    Definition sum' {Cat A} (u : mset (T (Cat,(A,A)))) : T (Cat,(A,A)) :=
       match u with
-        | nilne (u,xH) => u
-        | _ => sum i u
+      | nilne (u,xH) => u
+      | _ => sum i u
       end.
 
-    Definition is_sum  (u: T iTy) : @discr (mset (T iTy)) :=
-    match u with
-      | sum iTy j l => if eq_idx_bool j i then Is_op l else Is_nothing
-      | unit iTy j => if is_unit j   then Is_unit j else Is_nothing
-      | u => Is_nothing
+    Definition is_sum {Cat A B} (u: T Cat A B) : discr Cat A B :=
+    match u in T Cat A B return discr Cat A B with
+      | sum Cat A j l => if eq_idx_bool j i then Is_op _ l else Is_nothing _ 
+      | unit Cat A j => if is_unit j then Is_unit Cat A j else Is_nothing _
+      | u => Is_nothing _
     end.
 
-    Definition copy_mset n (l: mset (T iTy)): mset (T iTy) :=
+    Definition copy_mset {Cat A B} n (l: mset (T Cat A B)): mset (T Cat A B) :=
       match n with
         | xH => l
         | _ => nelist_map (fun vm => let '(v,m):=vm in (v,Pmult n m)) l
       end.
    
-    Definition return_sum  u n :=
-      match is_sum  u with
-        | Is_nothing => right (nilne (u,n))
-        | Is_op l' =>  right (copy_mset n l')
-        | Is_unit j => left j
+    Program Definition return_sum {Cat} {i1} u n : idx + mset (T (Cat,(i1,i1))):=
+      match is_sum u with
+        | Is_nothing _ => inr (nilne (u,n))
+        | Is_op _ l' =>  inr (copy_mset n l')
+        | Is_unit j => inl j
       end.
    
-    Definition add_to_sum u n (l : @m idx (mset (T iTy)))  :=
+    Definition add_to_sum {Cat i1} u n (l : idx + (mset (T (Cat,(i1,i1)))))  :=
       match is_sum  u with
-        | Is_nothing => comp (merge_msets compare) (nilne (u,n)) l
-        | Is_op l' => comp (merge_msets compare) (copy_mset n l') l
+        | Is_nothing _ => comp (merge_msets compare) (nilne (u,n)) l
+        | Is_op _ l' => comp (merge_msets compare) (copy_mset n l') l
         | Is_unit _ => l
     end.
 
 
-    Definition norm_msets_ norm  (l: mset (T iTy)) :=
+    Definition norm_msets_ {Cat} {i1} norm (l: mset (T (Cat,(i1,i1)))) : idx + mset (T(Cat,(i1,i1))):=
     fold_map'
     (fun un => let '(u,n) := un in  return_sum  (norm u) n)
     (fun un l => let '(u,n) := un in  add_to_sum  (norm u) n l) l.
@@ -272,70 +348,87 @@ Module ReifH.
   (** similar functions for products *)
 
   Section prds.
-    Variable iTy : idT.
     Variable i : idx.
     Variable is_unit : idx -> bool.
-    Definition prd'  (u: nelist (T iTy)): T iTy :=
+    
+    Definition prd' {Cat A B} (u: vAT Cat A B): T Cat A B :=
     match u with
-      | nilne u => u
-      | _ => prd i u
+      | vAnil u => u
+      | vAcons_ _ _ _ as u => prd i u
     end.
 
-    Definition is_prd (u: T iTy) : @discr (nelist (T iTy)) :=
-    match u with
-      | prd iTy j l => if eq_idx_bool j i then Is_op l else Is_nothing
-      | unit iTy j => if is_unit j  then Is_unit j else Is_nothing
-      | u => Is_nothing
+    Definition is_prd {Cat A B} (u: T Cat A B) : discr Cat A B :=
+    match u in T Cat A B return discr Cat A B with
+      | prd Cat A B j l => if eq_idx_bool j i then Is_op _ l else Is_nothing _
+      | unit j => if is_unit j  then Is_unit j else Is_nothing _
+      | u => Is_nothing _
     end.
  
    
-    Definition return_prd u :=
-      match is_prd u with
-        | Is_nothing => right (nilne (u))
-        | Is_op l' =>  right (l')
-        | Is_unit j => left j
+    Program Definition return_prd {Cat} {i1 i2} (u:T (Cat,(i1,i2))) : (idx * (i1=i2)) + vAT (Cat,(i1,i2)):=
+      match is_prd u in discr Cat A B return Cat A B = (Cat,(i1,i2)) -> (idx * (i1=i2)) + vAT (Cat,(i1,i2)) with
+        | Is_nothing _ => fun H => inr (vAnil (u))
+        | Is_op _ l' =>  fun H => inr (l')
+        | Is_unit j => fun H => inl (j,_)
+      end eq_refl.
+
+    Definition comp' {arr} {i1 i2 i3 : idx} {C D} (merge : arr i2 i3 -> arr i1 i2 -> arr i1 i3) (l : arr i2 i3) (l' : (D * (i1 = i2)) + arr i1 i2) : C + arr i1 i3 :=
+      match l' with
+      | inl (_,H) => inr (cast (fun i => arr i i3) (eq_sym H) l)
+      | inr l' => inr (merge l l')
       end.
    
-    Definition add_to_prd  u  (l : @m idx (nelist (T iTy)))  :=
-      match is_prd  u with
-        | Is_nothing => comp (@appne (T iTy)) (nilne (u)) l
-        | Is_op l' => comp (@appne (T iTy)) (l') l
-        | Is_unit _ => l
-      end.
+    Program Definition add_to_prd {Cat A B C} (u: T Cat B C):=
+      match is_prd u in @discr _ Cat A B return
+            forall (H:Cat A B = Cat B C) A,
+              (idx * (A = B)) + (vAT Cat A B) -> (idx * (A = C)) + (vAT Cat A C) with
+        | Is_nothing _=> fun H A l => comp' (arr:= fun i1 i2 => vAT (Cat,(i1,i2))) vAapp (vAnil u) l
+        | Is_op Cat A B''' l' => fun H A l => comp' (arr:= fun i1 i2 => vAT (Cat,(i1,i2))) vAapp l' l
+        | Is_unit _  => fun H A l => (cast (fun i : idx => (_ + vAT (Cat,(A,i)))%type) _ l)
+      end eq_refl A.
 
-    Definition norm_lists_ norm (l : nelist (T iTy)) :=
-    fold_map'
-    (fun u => return_prd  (norm u))
-    (fun u l => add_to_prd (norm u) l) l.
+    
+    
+    Definition norm_lists_ {Cat i1 i2} (norm: forall Cat A B, T Cat A B -> T Cat A B) (l : vAT (Cat,(i1,i2))) :=
+      fold_map_vA (fun Cat A B => match Cat A B with
+                             (Cat,(i1,i2))  => _ + _ end)%type
+                  (fun Cat' A' B' => match Cat' A' B' with
+                             (jCat,(j1,j2)) => 
+                             fun (u: T (jCat,(j1,j2))) => return_prd (norm _ u)
+                           end)
+                  (fun Cat i1 i2 i3 u l => add_to_prd (norm _ u) l) l.
 
 
   End prds.
 
 
-  Definition run_list {iTy} x := match x with
-                        | left n => nilne (unit iTy n)
-                        | right l => l
-                      end.
+  Definition run_list {Cat} {i1 i2} (x: _ + vAT (Cat,(i1,i2))) :=
+    match x with
+    | inl (n,H) => vAnil (cast (fun j => T (Cat,(i1,j))) H (unit Cat i1 n))
+    | inr l => l
+    end.
  
-  Definition norm_lists {iTy} (norm: T iTy -> T iTy) i l :=
-    let is_unit := is_unit_of iTy i in
+  Definition norm_lists {Cat} {i1 i2} (norm: forall Cat A B, T Cat A B -> T Cat A B ) i (l: vAT (Cat,(i1,i2))) :=
+    let is_unit := is_unit_of Cat i in
       run_list (norm_lists_ i is_unit norm l).
 
-  Definition run_msets {iTy} x := match x with
-                        | left n => nilne (unit iTy n, xH)
-                        | right l => l
+(* TODO: does this make sens? *)
+  
+  Definition run_msets {Cat} {i1} (x : (idx) + _) := match x with
+                        | inl (n,H) => nilne (cast (fun i => T (Cat,(i1,i))) H (unit Cat i1 n), xH)
+                        | inr l => l
                       end.
  
-  Definition norm_msets {iTy} (norm: T iTy -> T iTy) i l :=
-    let is_unit := is_unit_of iTy i in
+  Definition norm_msets {Cat} {i1} (norm: T (Cat,(i1,i1)) -> T _) i l :=
+    let is_unit := is_unit_of Cat i in
       run_msets (norm_msets_ i is_unit norm l).
  
-  Fixpoint norm {iTy} (u:T iTy) {struct u} : T iTy:=
+  Fixpoint norm {Cat A B} (u:T Cat A B) {struct u} : T Cat A B:=
     match u with
-      | sum iTy i l as u => if is_commutative iTy i then sum' i (norm_msets norm i l) else u
-      | prd iTy i l => prd' i (norm_lists norm i l)
-      | sym iTy i l => sym iTy i (vnorm l)
-      | unit iTy i as u => u
+      | sum Cat A B i l as u => if is_commutative Cat A B i then sum' i (norm_msets norm i l) else u
+      | prd Cat A B i l => prd' i (norm_lists norm i l)
+      | sym Cat A B i l => sym Cat A B i (vnorm l)
+      | unit Cat A B i as u => u
     end
   with vnorm i (l: vT i): vT i :=
     match l with
@@ -345,8 +438,8 @@ Module ReifH.
 
   (** ** Correctness *)
 
-  Lemma is_unit_of_Unit  : forall iTy (i j : idx),
-   is_unit_of iTy i j = true -> Unit (@eq (e_type iTy)) (bin_value (e_bin iTy i)) (eval (unit iTy j)).
+  Lemma is_unit_of_Unit  : forall Cat A B (i j : idx),
+   is_unit_of Cat A B i j = true -> Unit (@eq (e_type Cat A B)) (bin_value (e_bin Cat A B i)) (eval (unit Cat A B j)).
   Proof.
     intros. unfold is_unit_of in H.
     rewrite existsb_exists in H.
@@ -355,14 +448,14 @@ Module ReifH.
     simpl. destruct x. simpl. auto.
   Qed.
  
-  Instance Binvalue_Commutative iTy i (H : is_commutative iTy i = true) : Commutative eq (bin_value (e_bin iTy i) ).
+  Instance Binvalue_Commutative Cat A B i (H : is_commutative Cat A B i = true) : Commutative eq (bin_value (e_bin Cat A B i) ).
   Proof.
     unfold is_commutative in H.
     destruct bin_comm; auto.
     discriminate.
   Qed.
 
-  Instance Binvalue_Associative iTy i :Associative eq (bin_value (e_bin iTy i) ).
+  Instance Binvalue_Associative Cat A B i :Associative eq (bin_value (e_bin Cat A B i) ).
   Proof.
     destruct e_bin; auto.
   Qed.
@@ -378,17 +471,17 @@ Module ReifH.
 
   Hint Resolve is_unit_of_Unit.
   Section sum_correctness.
-    Variable iTy : idT.
+    Variable Cat A B : idT.
     Variable i : idx. (* The binary operator of the sum*)
     Variable is_unit : idx -> bool.
-    Hypothesis is_unit_sum_Unit : forall j, is_unit j = true -> @Unit _ eq (bin_value (e_bin iTy i)) (eval (unit iTy j)).
+    Hypothesis is_unit_sum_Unit : forall j, is_unit j = true -> @Unit _ eq (bin_value (e_bin Cat A B i)) (eval (unit Cat A B j)).
 
-    Inductive is_sum_spec_ind iTy: T iTy -> @discr (mset (T iTy)) -> Prop :=
+    Inductive is_sum_spec_ind Cat A B: T Cat A B -> @discr (mset (T Cat A B)) -> Prop :=
     | is_sum_spec_op : forall j l, j = i -> is_sum_spec_ind (sum j l) (Is_op l)
-    | is_sum_spec_unit : forall j, is_unit j = true ->  is_sum_spec_ind (unit iTy j) (Is_unit j)
+    | is_sum_spec_unit : forall j, is_unit j = true ->  is_sum_spec_ind (unit Cat A B j) (Is_unit j)
     | is_sum_spec_nothing : forall u, is_sum_spec_ind u (Is_nothing).
  
-    Lemma is_sum_spec (u:T iTy) : is_sum_spec_ind u (is_sum i is_unit u).
+    Lemma is_sum_spec (u:T Cat A B) : is_sum_spec_ind u (is_sum i is_unit u).
     Proof.
       unfold is_sum; destruct u; intros; try constructor.
       -destruct eq_idx_bool eqn:eq1. 2: now constructor.
@@ -396,32 +489,32 @@ Module ReifH.
       -case_eq (is_unit j); intros; try constructor. auto.
     Qed.
 
-    Instance assoc :   @Associative _ eq (bin_value (e_bin iTy i)).
+    Instance assoc :   @Associative _ eq (bin_value (e_bin Cat A B i)).
     Proof.
-      destruct (e_bin iTy i). simpl. assumption.
+      destruct (e_bin Cat A B i). simpl. assumption.
     Qed.
     (*Instance proper :   Proper (R ==> R ==> R) (Bin.value (e_bin i)).
     Proof.
       destruct (e_bin i). simpl. assumption.
     Qed.*)
-    Hypothesis comm : @Commutative _ eq (bin_value (e_bin iTy i)).
+    Hypothesis comm : @Commutative _ eq (bin_value (e_bin Cat A B i)).
 
-    Lemma sum'_sum : forall  (l: mset (T iTy)),  eval (sum' i l) = eval (sum i l) .
+    Lemma sum'_sum : forall  (l: mset (T Cat A B)),  eval (sum' i l) = eval (sum i l) .
     Proof.
       intros [[a n] | [a n] l]; destruct n;  simpl; reflexivity.
     Qed.
 
-    Lemma eval_sum_nil (x:T iTy):
+    Lemma eval_sum_nil (x:T Cat A B):
       eval (sum i (nilne (x,xH))) = (eval x).
     Proof. rewrite <- sum'_sum. reflexivity.   Qed.
      
-    Lemma eval_sum_cons : forall n a (l: mset (T iTy)),
-      (eval (sum i ((a,n):::l))) = (bin_value (e_bin iTy i) (@copy _ (bin_value (e_bin iTy i)) n (eval a)) (eval (sum i l))).
+    Lemma eval_sum_cons : forall n a (l: mset (T Cat A B)),
+      (eval (sum i ((a,n):::l))) = (bin_value (e_bin Cat A B i) (@copy _ (bin_value (e_bin Cat A B i)) n (eval a)) (eval (sum i l))).
     Proof.
       intros n a [[? ? ]|[b m] l]; simpl; reflexivity.
     Qed.
    
-    Inductive compat_sum_unit : @m idx (mset (T iTy)) -> Prop :=
+    Inductive compat_sum_unit : @m idx (mset (T Cat A B)) -> Prop :=
     | csu_left : forall x,  is_unit x = true->  compat_sum_unit  (left x)
     | csu_right : forall m, compat_sum_unit (right m).
 
@@ -434,11 +527,11 @@ Module ReifH.
     Lemma compat_sum_unit_add : forall x n h,
         compat_sum_unit  h ->
         compat_sum_unit
-          (add_to_sum i (is_unit_of iTy i) x n
+          (add_to_sum i (is_unit_of Cat A B i) x n
                       h).
     Proof.
       unfold add_to_sum;intros; inversion H;
-        case_eq  (is_sum i (is_unit_of iTy i) x);
+        case_eq  (is_sum i (is_unit_of Cat A B i) x);
         intros; simpl; try constructor || eauto. apply H0.
     Qed.
 
@@ -447,8 +540,8 @@ Module ReifH.
     Hint Extern 5 (?x = ?x) => reflexivity.
     Hint Extern 5 (bin_value ?x ?y = bin_value ?y ?x) => apply bin_comm.
    
-    Lemma eval_merge_bin : forall (h k: mset (T iTy)),
-      eval (sum i (merge_msets compare h k)) = bin_value (e_bin iTy i) (eval (sum i h)) (eval (sum i k)).
+    Lemma eval_merge_bin : forall (h k: mset (T Cat A B)),
+      eval (sum i (merge_msets compare h k)) = bin_value (e_bin Cat A B i) (eval (sum i h)) (eval (sum i k)).
     Proof.
       induction h as [[a n]|[a n] h IHh]; intro k.
       -simpl.
@@ -473,7 +566,7 @@ Module ReifH.
     Qed.
 
  
-    Lemma copy_mset' n (l: mset (T iTy)):  copy_mset n l = nelist_map (fun vm => let '(v,m):=vm in (v,Pmult n m)) l.
+    Lemma copy_mset' n (l: mset (T Cat A B)):  copy_mset n l = nelist_map (fun vm => let '(v,m):=vm in (v,Pmult n m)) l.
     Proof.
       unfold copy_mset.  destruct n; try reflexivity.
      
@@ -481,7 +574,7 @@ Module ReifH.
     Qed.
    
    
-    Lemma copy_mset_succ  n (l: mset (T iTy)):  eval (sum i (copy_mset (Pos.succ n) l)) = bin_value (e_bin iTy i) (eval (sum i l)) (eval (sum i (copy_mset n l))).
+    Lemma copy_mset_succ  n (l: mset (T Cat A B)):  eval (sum i (copy_mset (Pos.succ n) l)) = bin_value (e_bin Cat A B i) (eval (sum i l)) (eval (sum i (copy_mset n l))).
     Proof.
       rewrite 2 copy_mset'.
      
@@ -493,7 +586,7 @@ Module ReifH.
        rewrite law_comm . rewrite <- !law_assoc. f_equal. apply law_comm.
     Qed.
 
-    Lemma copy_mset_copy : forall n  (m : mset (T iTy)), eval (sum i (copy_mset n m)) = @copy _ (bin_value (e_bin iTy i)) n (eval (sum i m)).
+    Lemma copy_mset_copy : forall n  (m : mset (T Cat A B)), eval (sum i (copy_mset n m)) = @copy _ (bin_value (e_bin Cat A B i)) n (eval (sum i m)).
     Proof.
       induction n using Pind; intros.
      
@@ -502,14 +595,14 @@ Module ReifH.
     Qed.
    
     Instance compat_sum_unit_Unit : forall p, compat_sum_unit (left p) ->
-      @Unit _ eq (bin_value (e_bin iTy i)) (eval (unit iTy p)).
+      @Unit _ eq (bin_value (e_bin Cat A B i)) (eval (unit Cat A B p)).
     Proof.
       intros.
       inversion H. subst.  auto.
     Qed.
   
     Lemma copy_n_unit : forall j n, is_unit j = true ->
-      eval (unit iTy j) = @copy _ (bin_value (e_bin iTy i)) n (eval (unit iTy j)).
+      eval (unit Cat A B j) = @copy _ (bin_value (e_bin Cat A B i)) n (eval (unit Cat A B j)).
     Proof.
       intros.
       induction n using Prect.
@@ -531,7 +624,7 @@ Module ReifH.
 
     Lemma z1 : forall n x,
       eval (sum i (run_msets (return_sum i (is_unit) x n )))
-      = @copy _ (bin_value (e_bin iTy i)) n (eval x).
+      = @copy _ (bin_value (e_bin Cat A B i)) n (eval x).
     Proof.
       intros. unfold return_sum.  unfold run_msets.
       destruct (is_sum_spec x); intros; subst.
@@ -544,7 +637,7 @@ Module ReifH.
       eval (sum i ( run_msets
         (add_to_sum i (is_unit) u n x)))
       = 
-      bin_value (e_bin iTy i) (@copy _ (bin_value (e_bin iTy i))  n (eval u)) (eval (sum i (run_msets x))).
+      bin_value (e_bin Cat A B i) (@copy _ (bin_value (e_bin Cat A B i))  n (eval u)) (eval (sum i (run_msets x))).
     Proof.
       intros u n x Hix .
       unfold add_to_sum.
@@ -560,14 +653,14 @@ Module ReifH.
     Qed.
   End sum_correctness.
   
-  Lemma eval_norm_msets iTy i norm
-    (Comm : Commutative eq (bin_value (e_bin iTy i)))
-    (Hnorm: forall (u : T iTy), eval (norm u) = eval u) : forall h, eval (sum i (norm_msets norm i h)) = eval (sum i h).
+  Lemma eval_norm_msets Cat A B i norm
+    (Comm : Commutative eq (bin_value (e_bin Cat A B i)))
+    (Hnorm: forall (u : T Cat A B), eval (norm u) = eval u) : forall h, eval (sum i (norm_msets norm i h)) = eval (sum i h).
   Proof.
     unfold norm_msets.
     assert (H :
-      forall h : mset (T iTy),
-        eval (sum i (run_msets (norm_msets_ i (is_unit_of iTy i) norm h))) =  eval (sum i h) /\ compat_sum_unit (is_unit_of iTy i) (norm_msets_ i (is_unit_of iTy i) norm h)).
+      forall h : mset (T Cat A B),
+        eval (sum i (run_msets (norm_msets_ i (is_unit_of Cat A B i) norm h))) =  eval (sum i h) /\ compat_sum_unit (is_unit_of Cat A B i) (norm_msets_ i (is_unit_of Cat A B i) norm h)).
       
     -induction h as [[a n] | [a n] h [IHh IHh']]; simpl norm_msets_; split.
      +rewrite z1 by auto.  rewrite Hnorm . reflexivity.
@@ -581,47 +674,47 @@ Module ReifH.
   (** auxiliary lemmas about products  *)
 
   Section prd_correctness.
-    Variable iTy : idT. 
+    Variable Cat A B : idT. 
     Variable i : idx.
     Variable is_unit : idx -> bool.
-    Hypothesis is_unit_prd_Unit : forall j, is_unit j = true->  @Unit _ eq (bin_value (e_bin iTy i)) (eval (unit iTy j)).
+    Hypothesis is_unit_prd_Unit : forall j, is_unit j = true->  @Unit _ eq (bin_value (e_bin Cat A B i)) (eval (unit Cat A B j)).
 
-    Inductive is_prd_spec_ind iTy : T iTy ->  @discr (nelist (T iTy)) -> Prop :=
+    Inductive is_prd_spec_ind Cat A B : T Cat A B ->  @discr (nelist (T Cat A B)) -> Prop :=
     | is_prd_spec_op :
       forall j l, j = i -> is_prd_spec_ind (prd j l) (Is_op l)
     | is_prd_spec_unit :
-      forall j, is_unit j = true ->  is_prd_spec_ind (unit iTy j) (Is_unit j)
+      forall j, is_unit j = true ->  is_prd_spec_ind (unit Cat A B j) (Is_unit j)
     | is_prd_spec_nothing :
       forall u, is_prd_spec_ind u (Is_nothing).
    
-    Lemma is_prd_spec (u : T iTy ) : is_prd_spec_ind u (is_prd i is_unit u).
+    Lemma is_prd_spec (u : T Cat A B ) : is_prd_spec_ind u (is_prd i is_unit u).
     Proof.
       unfold is_prd; destruct u; intros; try constructor.
       -case (eq_idx_spec); intros; subst;  try constructor; auto.
       -case_eq (is_unit j); intros; try constructor; auto.
     Qed.
 
-    Lemma prd'_prd : forall (l: nelist (T iTy)), eval (prd' i l) = eval (prd i l).
+    Lemma prd'_prd : forall (l: nelist (T Cat A B)), eval (prd' i l) = eval (prd i l).
     Proof.
       intros  [?|? [|? ?]]; simpl; reflexivity.
     Qed.
    
    
-    Lemma eval_prd_nil (x: T iTy):  eval (prd i (nilne x)) = eval x.
+    Lemma eval_prd_nil (x: T Cat A B):  eval (prd i (nilne x)) = eval x.
     Proof.
       rewrite <- prd'_prd. simpl. reflexivity.
     Qed.
-    Lemma eval_prd_cons a : forall (l: nelist (T iTy)), eval (prd i (a:::l)) = bin_value (e_bin iTy i) (eval a) (eval (prd i l)).
+    Lemma eval_prd_cons a : forall (l: nelist (T Cat A B)), eval (prd i (a:::l)) = bin_value (e_bin Cat A B i) (eval a) (eval (prd i l)).
     Proof.
       intros  [|b l]; simpl; reflexivity.
     Qed.
-    Lemma eval_prd_app : forall (h k: nelist (T iTy)), eval (prd i (appne h k)) = bin_value (e_bin iTy i) (eval (prd i h)) (eval (prd i k)).
+    Lemma eval_prd_app : forall (h k: nelist (T Cat A B)), eval (prd i (appne h k)) = bin_value (e_bin Cat A B i) (eval (prd i h)) (eval (prd i k)).
     Proof.
       induction h; intro k. simpl; try reflexivity.
       simpl appne.  rewrite  2 eval_prd_cons, IHh, law_assoc. reflexivity.
     Qed.
 
-    Inductive compat_prd_unit : @m idx (nelist (T iTy)) -> Prop :=
+    Inductive compat_prd_unit : @m idx (nelist (T Cat A B)) -> Prop :=
     | cpu_left : forall x,  is_unit  x = true -> compat_prd_unit  (left x)
     | cpu_right : forall m, compat_prd_unit (right m)
     .
@@ -649,13 +742,13 @@ Module ReifH.
 
    
     Instance compat_prd_Unit : forall p, compat_prd_unit (left p) ->
-      @Unit _ eq (bin_value (e_bin iTy i)) (eval (unit iTy p)).
+      @Unit _ eq (bin_value (e_bin Cat A B i)) (eval (unit Cat A B p)).
     Proof.
       intros.
       inversion H; subst. apply is_unit_prd_Unit. assumption.
     Qed.
 
-    Lemma z0' : forall l (r: @m idx (nelist (T iTy))), compat_prd_unit r ->
+    Lemma z0' : forall l (r: @m idx (nelist (T Cat A B))), compat_prd_unit r ->
       eval (prd i (run_list (comp (@appne _) l r))) = eval (prd i ((appne (l) (run_list r)))).
     Proof.
       intros.
@@ -665,14 +758,14 @@ Module ReifH.
       apply compat_prd_Unit in H. rewrite law_neutral_right. reflexivity.
     Qed.
  
-    Lemma z1' (a:T iTy) :  eval (prd i (run_list (return_prd i is_unit a))) =  eval (prd i (nilne a)).
+    Lemma z1' (a:T Cat A B) :  eval (prd i (run_list (return_prd i is_unit a))) =  eval (prd i (nilne a)).
     Proof.
       intros. unfold return_prd.  unfold run_list.
       case (is_prd_spec); intros; subst; reflexivity.
     Qed.
     Lemma z2' : forall  u  x, compat_prd_unit  x ->
       eval (prd i ( run_list
-        (add_to_prd i is_unit u x))) =  bin_value (e_bin iTy i) (eval u) (eval (prd i (run_list x))).
+        (add_to_prd i is_unit u x))) =  bin_value (e_bin Cat A B i) (eval u) (eval (prd i (run_list x))).
     Proof.
       intros u x Hix.
       unfold add_to_prd.
@@ -687,13 +780,13 @@ Module ReifH.
 
 
 
-  Lemma eval_norm_lists iTy i (Hnorm: forall (u : T iTy), eval (norm u) = eval u) : forall h : (nelist (T iTy)), eval (prd i (norm_lists norm i h)) = eval (prd i h).
+  Lemma eval_norm_lists Cat A B i (Hnorm: forall (u : T Cat A B), eval (norm u) = eval u) : forall h : (nelist (T Cat A B)), eval (prd i (norm_lists norm i h)) = eval (prd i h).
   Proof.
     unfold norm_lists.
-    assert (H :  forall h : nelist (T iTy),
-      eval (prd i (run_list (norm_lists_ i (is_unit_of iTy i) norm h))) =
+    assert (H :  forall h : nelist (T Cat A B),
+      eval (prd i (run_list (norm_lists_ i (is_unit_of Cat A B i) norm h))) =
       eval (prd i h)
-      /\ compat_prd_unit (is_unit_of iTy i) (norm_lists_ i (is_unit_of iTy i) norm h)).
+      /\ compat_prd_unit (is_unit_of Cat A B i) (norm_lists_ i (is_unit_of Cat A B i) norm h)).
     {
       induction h as [a | a h [IHh IHh']]; simpl norm_lists_; split.
       -rewrite z1'. 2:now eauto. simpl.  apply Hnorm.
@@ -706,12 +799,12 @@ Module ReifH.
 
   (** correctness of the normalisation function *)
 
-  Theorem eval_norm: forall iTy (u: T iTy), eval (norm u) = eval u
+  Theorem eval_norm: forall Cat A B (u: T Cat A B), eval (norm u) = eval u
     with eval_norm_aux: forall arTy ret (l: vT arTy) (f: type_of_ar arTy ret),
       eval_aux (vnorm l) f = eval_aux l f.
   Proof.
-    induction u as [ iTy p m | iTY p l | iTy ? | iTy ?];  cbn [norm].
-    -case_eq (is_commutative iTy p); intros.
+    induction u as [ Cat A B p m | iTY p l | Cat A B ? | Cat A B ?];  cbn [norm].
+    -case_eq (is_commutative Cat A B p); intros.
      +rewrite sum'_sum.
       apply eval_norm_msets; auto.
      +reflexivity.
@@ -727,13 +820,13 @@ Module ReifH.
 
   (** corollaries, for goal normalisation or decision *)
 
-  Lemma normalise : forall iTy (u v: T iTy), eval (norm u) = eval (norm v) -> eval u = eval v.
+  Lemma normalise : forall Cat A B (u v: T Cat A B), eval (norm u) = eval (norm v) -> eval u = eval v.
   Proof. intros ? u v. rewrite 2 eval_norm. trivial. Qed.
    
-  Lemma compare_reflect_eq iTy (u v : T iTy) : compare u v = Eq -> eval u = eval v.
+  Lemma compare_reflect_eq Cat A B (u v : T Cat A B) : compare u v = Eq -> eval u = eval v.
   Proof. case (tcompare_weak_spec u v); intros; try congruence. Qed.
 
-  Lemma decide iTy (u v: T iTy): compare (norm u) (norm v) = Eq -> eval u = eval v.
+  Lemma decide Cat A B (u v: T Cat A B): compare (norm u) (norm v) = Eq -> eval u = eval v.
   Proof. intros H. apply normalise. apply compare_reflect_eq. apply H. Qed.
 
   (* Lemma lift_normalise {S} {H : AAC_lift S R}: *)
